Integrate gcm_decrypt with a few assumes left

vale/code/arch/x64/interop/GCMdecrypt_stdcalls.fst
@@ -4,6 +4,7 @@ open Vale.Stdcalls.GCMdecrypt
 open Vale.AsLowStar.MemoryHelpers
 open X64.MemoryAdapters
 module V = X64.Vale.Decls
+open Simplify_Sha
 open Gcm_simplify
 open GCM_helpers
 
@@ -11,7 +12,7 @@ open GCM_helpers
 
 let math_aux (n:nat) : Lemma (n * 1 == n) = ()
 
-let gcm128_decrypt key cipher_b cipher_num auth_b auth_num iv_b out_b tag_b keys_b =
+let gcm128_decrypt_stdcall key cipher_b cipher_num auth_b auth_num iv_b out_b tag_b keys_b =
   let h0 = get() in
   bytes_to_quad_size_no_extra_bytes (UInt64.v cipher_num);
   bytes_to_quad_size_no_extra_bytes (UInt64.v auth_num);
@@ -42,6 +43,26 @@ let gcm128_decrypt key cipher_b cipher_num auth_b auth_num iv_b out_b tag_b keys
   Classical.forall_intro (bounded_buffer_addrs TUInt8 TUInt128 h0 auth_b);
   Classical.forall_intro (bounded_buffer_addrs TUInt8 TUInt128 h0 out_b);
 
+  let lemma_uv_key () : Lemma
+    (let db = get_downview keys_b in
+      length_aux keys_b;
+      let ub = UV.mk_buffer db Views.up_view128 in
+      Seq.equal (UV.as_seq h0 ub) (key_to_round_keys_LE AES_128 (Ghost.reveal key)))
+    = length_aux keys_b;
+      let db = get_downview keys_b in
+      let ub = UV.mk_buffer db Views.up_view128 in
+      le_bytes_to_seq_quad32_to_bytes (key_to_round_keys_LE AES_128 (Ghost.reveal key));
+      assert (Seq.equal (le_bytes_to_seq_quad32 (seq_uint8_to_seq_nat8 (B.as_seq h0 keys_b)))
+         (key_to_round_keys_LE AES_128 (Ghost.reveal key)));   
+      calc (==) {
+        le_bytes_to_seq_quad32 (seq_uint8_to_seq_nat8 (B.as_seq h0 keys_b));
+        (==) { lemma_seq_nat8_le_seq_quad32_to_bytes_uint32 keys_b h0 }
+        le_bytes_to_seq_quad32 (seq_uint8_to_seq_nat8 (seq_nat8_to_seq_uint8 (le_seq_quad32_to_bytes (UV.as_seq h0 ub))));
+        (==) { le_bytes_to_seq_quad32_to_bytes (UV.as_seq h0 ub) }
+        UV.as_seq h0 ub;
+      }
+
+  in lemma_uv_key ();
   let x, _ = gcm128_decrypt key cipher_b cipher_num auth_b auth_num iv_b keys_b out_b tag_b () in
 
   let h1 = get() in
@@ -55,7 +76,7 @@ let gcm128_decrypt key cipher_b cipher_num auth_b auth_num iv_b out_b tag_b keys
   x
 
 
-let gcm256_decrypt key cipher_b cipher_num auth_b auth_num iv_b out_b tag_b keys_b =
+let gcm256_decrypt_stdcall key cipher_b cipher_num auth_b auth_num iv_b out_b tag_b keys_b =
   let h0 = get() in
   bytes_to_quad_size_no_extra_bytes (UInt64.v cipher_num);
   bytes_to_quad_size_no_extra_bytes (UInt64.v auth_num);
@@ -85,6 +106,27 @@ let gcm256_decrypt key cipher_b cipher_num auth_b auth_num iv_b out_b tag_b keys
   Classical.forall_intro (bounded_buffer_addrs TUInt8 TUInt128 h0 cipher_b);
   Classical.forall_intro (bounded_buffer_addrs TUInt8 TUInt128 h0 auth_b);
   Classical.forall_intro (bounded_buffer_addrs TUInt8 TUInt128 h0 out_b);
+
+  let lemma_uv_key () : Lemma
+    (let db = get_downview keys_b in
+      length_aux2 keys_b;
+      let ub = UV.mk_buffer db Views.up_view128 in
+      Seq.equal (UV.as_seq h0 ub) (key_to_round_keys_LE AES_256 (Ghost.reveal key)))
+    = length_aux2 keys_b;
+      let db = get_downview keys_b in
+      let ub = UV.mk_buffer db Views.up_view128 in
+      le_bytes_to_seq_quad32_to_bytes (key_to_round_keys_LE AES_256 (Ghost.reveal key));
+      assert (Seq.equal (le_bytes_to_seq_quad32 (seq_uint8_to_seq_nat8 (B.as_seq h0 keys_b)))
+         (key_to_round_keys_LE AES_256 (Ghost.reveal key)));   
+      calc (==) {
+        le_bytes_to_seq_quad32 (seq_uint8_to_seq_nat8 (B.as_seq h0 keys_b));
+        (==) { lemma_seq_nat8_le_seq_quad32_to_bytes_uint32 keys_b h0 }
+        le_bytes_to_seq_quad32 (seq_uint8_to_seq_nat8 (seq_nat8_to_seq_uint8 (le_seq_quad32_to_bytes (UV.as_seq h0 ub))));
+        (==) { le_bytes_to_seq_quad32_to_bytes (UV.as_seq h0 ub) }
+        UV.as_seq h0 ub;
+      }
+
+  in lemma_uv_key ();
   
   let x, _ = gcm256_decrypt key cipher_b cipher_num auth_b auth_num iv_b keys_b out_b tag_b () in
 
